#
# Copyright (c) 2012 di.me Consortium
# 
# All rights reserved, licensed under either CC-BY or BSD.
#
# You are free:
#  * to Share - to copy, distribute and transmit the work
#  * to Remix - to adapt the work
# Under the following conditions:
#  * Attribution - You must attribute the work in the manner specified by the author
#    or licensor (but not in any way that suggests that they endorse you or your use 
#    of the work).
#
# Redistribution and use in source and binary forms, with or without modification, 
# are permitted provided that the following conditions are met:
#  * Redistributions of source code must retain the above copyright notice, this 
#    list of conditions and the following disclaimer.
#  * Redistributions in binary form must reproduce the above copyright notice, this 
#    list of conditions and the following disclaimer in the documentation and/or 
#    other materials provided with the distribution.
#  * Neither the names of the authors nor the names of contributors may
#    be used to endorse or promote products derived from this ontology without 
#    specific prior written permission.
#
# THIS ONTOLOGY IS PROVIDED BY THE AUTHOR ``AS IS'' AND ANY EXPRESS OR
# IMPLIED WARRANTIES, INCLUDING, BUT NOT LIMITED TO, THE IMPLIED WARRANTIES
# OF MERCHANTABILITY AND FITNESS FOR A PARTICULAR PURPOSE ARE DISCLAIMED.
# IN NO EVENT SHALL THE AUTHOR BE LIABLE FOR ANY DIRECT, INDIRECT,
# INCIDENTAL, SPECIAL, EXEMPLARY, OR CONSEQUENTIAL DAMAGES (INCLUDING, BUT
# NOT LIMITED TO, PROCUREMENT OF SUBSTITUTE GOODS OR SERVICES; LOSS OF USE,
# DATA, OR PROFITS; OR BUSINESS INTERRUPTION) HOWEVER CAUSED AND ON ANY
# THEORY OF LIABILITY, WHETHER IN CONTRACT, STRICT LIABILITY, OR TORT
# (INCLUDING NEGLIGENCE OR OTHERWISE) ARISING IN ANY WAY OUT OF THE USE OF
# THIS ONTOLOGY, EVEN IF ADVISED OF THE POSSIBILITY OF SUCH DAMAGE.
#

@prefix xsd:     <http://www.w3.org/2001/XMLSchema#> .
@prefix pimo:    <http://www.semanticdesktop.org/ontologies/2007/11/01/pimo#> .
@prefix ddo:	<http://www.semanticdesktop.org/ontologies/2011/10/05/ddo#> .
@prefix rdfs:    <http://www.w3.org/2000/01/rdf-schema#> .
@prefix nrl:    <http://www.semanticdesktop.org/ontologies/2007/08/15/nrl#> .
@prefix nie:     <http://www.semanticdesktop.org/ontologies/2007/01/19/nie#> .
@prefix nao:     <http://www.semanticdesktop.org/ontologies/2007/08/15/nao#> .
@prefix rdf:     <http://www.w3.org/1999/02/22-rdf-syntax-ns#> .

<http://www.semanticdesktop.org/ontologies/2011/10/05/ddo> {
	# Classes
	ddo:Device
		a		rdfs:Class ;
		rdfs:subClassOf nie:DataSource ;
		rdfs:comment "A computerised device or gadget containing digital information, e.g. desktops, laptops, tablets and smart phones. Subclass of nie:DataSource, as a source of personal information." ;
		rdfs:label "Device" .

	ddo:Network
		a		rdfs:Class ;
		rdfs:comment "A telecommunications network, connecting a collection of terminals, links and nodes which connect together to enable telecommunication between terminal users. Includes wired and wireless computer networks and cellular networks." ;
		rdfs:label "Network" .
		
	ddo:CellularNetwork
		a		rdfs:Class ;
		rdfs:comment "A cell-based radio network that enables mobile telephony." ;
		rdfs:label "CellularNetwork" ;
		rdfs:subClassOf ddo:Network .
	
	ddo:ComputerNetwork
		a		rdfs:Class ;
		rdfs:comment "A communication channel that enables the interconnection and sharing of resources and information between a collection of hardware components and computers." ;
		rdfs:label "ComputerNetwork" ;
		rdfs:subClassOf ddo:Network .
	
	ddo:LocalAreaNetwork
		a		rdfs:Class ;
		rdfs:comment "A Local Area Network (LAN) is a private computer network that enables communication among computerised devices in a limited area.";
		rdfs:label "LocalAreaNetwork" ;
		rdfs:subClassOf ddo:ComputerNetwork .

	ddo:PersonalAreaNetwork
		a		rdfs:Class ;
		rdfs:comment "A Personal Area Network (PAN) is a computer network that enables intrapersonal communication amongst personal computerised devices. PANs can also be used to connect to a higher level network (including the Internet)." ;
		rdfs:label "PersonalAreaNetwork" ;
		rdfs:subClassOf ddo:ComputerNetwork .
	
	ddo:Bluetooth
		a		rdfs:Class ;
		rdfs:comment "Bluetooth networks refer to personal area networks created between computerised devices in order to exchange data over short distances." ;
		rdfs:label "Bluetooth" ;
		rdfs:subClassOf ddo:PersonalAreaNetwork .
		
	ddo:WiFi
		a		rdfs:Class ;
		rdfs:comment "A wireless local area network that allows computerised devices to exchange data wirelessly. Devices can connect to a wireless network via a wireless network access point. " ;
		rdfs:label "WiFi" ;
		rdfs:subClassOf ddo:LocalAreaNetwork .
	
	ddo:Ethernet
		a		rdfs:Class ;
		rdfs:comment "A wired local area network enabling computerised devices to exchange streams of data." ;
		rdfs:label "Ethernet" ;
		rdfs:subClassOf ddo:LocalAreaNetwork .
	
	ddo:GSM
		a		rdfs:Class ;
		rdfs:comment "Global System for Mobile Communications (GSM) is a second generation (2G) of standards for digital cellular networks." ;
		rdfs:label "GSM" ;
		rdfs:subClassOf ddo:CellularNetwork .
	
	<http://www.semanticdesktop.org/ontologies/2011/10/05/ddo#3G>
		a		rdfs:Class ;
		rdfs:comment "3rd generation mobile telecommunications (3G) is a third generation of standards for digital cellular networks." ;
		rdfs:label "3G" ;
		rdfs:subClassOf ddo:CellularNetwork .
		
	# Properties
    ddo:owns
          a       rdf:Property ;
          rdfs:comment "Defines an ownership relationship between a person and a computerised device." ;
          rdfs:domain 	pimo:Person ;
          rdfs:label "owns" ;
          rdfs:range ddo:Device .
		  
    ddo:deviceName
          a       rdf:Property ;
          rdfs:comment "Represents a person-defined name for a device." ;
          rdfs:domain 	ddo:Device ;
          rdfs:label "deviceName" ;
          rdfs:range xsd:string ;
		  rdfs:subPropertyOf nao:personalIdentifier .
		  
	
	ddo:deviceIdentifier
          a       rdf:Property ;
          rdfs:comment "Represents the internal identifier for a device." ;
          rdfs:domain 	ddo:Device ;
          rdfs:label "deviceIdentifier" ;
          rdfs:range xsd:string ;
		  rdfs:subPropertyOf nao:identifier .
	
	ddo:knownNetwork
          a       rdf:Property ;
          rdfs:comment "Establishes a relationship between networks that have at some point in time (past or present) been either connected or in range of a device." ;
          rdfs:domain 	ddo:Device ;
          rdfs:label "knownNetwork" ;
          rdfs:range ddo:Network .
			  
    	  
    ddo:networkID
          a       rdf:Property ;
          rdfs:comment "Attaches a name to a network. Use ddo:accessPointID and ddo:cellID for more specific identification." ;
          rdfs:domain 	ddo:Network;
          rdfs:label "networkID" ;
          rdfs:range xsd:string .		 		 		  				

	ddo:sourceDevice
          a       rdf:Property ;
          rdfs:comment "Identifies the device that is, or has, enabled a specific Bluetooth network." ;
          rdfs:domain 	ddo:Bluetooth ;
          rdfs:label "Source Device" ;
          rdfs:range ddo:Device .
	
	ddo:accessPointID
          a       rdf:Property ;
          rdfs:comment "Attaches a human-readable name to a computer network." ;
          rdfs:domain 	ddo:ComputerNetwork ;
          rdfs:label "accessPointID" ;
          rdfs:subPropertyOf ddo:networkID .
		  
    ddo:ipAddress
          a       rdf:Property ;
          rdfs:comment "Defines the known IP address for a computer network." ;
          rdfs:domain 	ddo:ComputerNetwork ;
          rdfs:label "ipAddress" ;
          rdfs:range xsd:string .
		  
    ddo:macAddress
          a       rdf:Property ;
          rdfs:comment "Defines the known mac address for a computer network." ;
          rdfs:domain 	ddo:ComputerNetwork ;
          rdfs:label "macAddress" ;
          rdfs:range xsd:string .
		  
    
    ddo:cellID
          a       rdf:Property ;
          rdfs:comment "Identifies the known cells (tower) that is, or has, enabled a specific cellular network." ;
          rdfs:domain 	ddo:CellularNetwork;
          rdfs:subPropertyOf ddo:networkID ;
		  rdfs:label "cellID" .		 		 		  				
		  
	ddo:carrierID
          a       rdf:Property ;
          rdfs:comment "Attaches a human-readable name to a cellular network." ;
          rdfs:domain 	ddo:CellularNetwork;
          rdfs:label "cellID" ;
          rdfs:range xsd:string .		 		 	

	ddo:isSecure
          a       rdf:Property ;
          rdfs:comment "States whether the network is secure (requires some form of authentication) or otherwise." ;
          rdfs:domain 	ddo:Network;
          rdfs:label "is secure" ;
          rdfs:range xsd:boolean .		 		 	
}

<http://www.semanticdesktop.org/ontologies/2011/10/05/ddo/metadata> {
    <http://www.semanticdesktop.org/ontologies/2011/10/05/ddo/metadata>
          a       nrl:GraphMetadata ;
          nrl:coreGraphMetadataFor <http://www.semanticdesktop.org/ontologies/2011/10/05/ddo> .


    <http://www.semanticdesktop.org/ontologies/2011/10/05/ddo>
          a       nrl:Ontology , nrl:DocumentGraph ;
          nao:hasDefaultNamespace "http://www.semanticdesktop.org/ontologies/2011/10/05/ddo#" ;
          nao:hasDefaultNamespaceAbbreviation "ddo" ;
          nao:lastModified "2012-10-25T00:00:00Z" ;
          nao:serializationLanguage "TriG" ;
          nao:status "Testing" ;
          nrl:updatable "0" ;
		  nao:creator <http://www.deri.ie/about/team/member/simon_scerri> ;
          nao:contributor <http://www.deri.ie/users/ismael-rivera> ;
		  nao:version "1.0" ;
          nao:prefLabel "digital.me Device Ontology" ;
          nao:description "The DDO provides vocabulary for the representation of personal devices, including personal computers, smartphones, gadgets; and their identifiers and characteristics, including network connections." .
}