#
# Copyright (c) 2012 di.me Consortium
#
# All rights reserved, licensed under either CC-BY or BSD.
#
# You are free:
#  * to Share - to copy, distribute and transmit the work
#  * to Remix - to adapt the work
# Under the following conditions:
#  * Attribution - You must attribute the work in the manner specified by the author
#    or licensor (but not in any way that suggests that they endorse you or your use 
#    of the work).
#
# Redistribution and use in source and binary forms, with or without modification, 
# are permitted provided that the following conditions are met:
#  * Redistributions of source code must retain the above copyright notice, this 
#    list of conditions and the following disclaimer.
#  * Redistributions in binary form must reproduce the above copyright notice, this 
#    list of conditions and the following disclaimer in the documentation and/or 
#    other materials provided with the distribution.
#  * Neither the names of the authors nor the names of contributors may
#    be used to endorse or promote products derived from this ontology without 
#    specific prior written permission.
#
# THIS ONTOLOGY IS PROVIDED BY THE AUTHOR ``AS IS'' AND ANY EXPRESS OR
# IMPLIED WARRANTIES, INCLUDING, BUT NOT LIMITED TO, THE IMPLIED WARRANTIES
# OF MERCHANTABILITY AND FITNESS FOR A PARTICULAR PURPOSE ARE DISCLAIMED.
# IN NO EVENT SHALL THE AUTHOR BE LIABLE FOR ANY DIRECT, INDIRECT,
# INCIDENTAL, SPECIAL, EXEMPLARY, OR CONSEQUENTIAL DAMAGES (INCLUDING, BUT
# NOT LIMITED TO, PROCUREMENT OF SUBSTITUTE GOODS OR SERVICES; LOSS OF USE,
# DATA, OR PROFITS; OR BUSINESS INTERRUPTION) HOWEVER CAUSED AND ON ANY
# THEORY OF LIABILITY, WHETHER IN CONTRACT, STRICT LIABILITY, OR TORT
# (INCLUDING NEGLIGENCE OR OTHERWISE) ARISING IN ANY WAY OUT OF THE USE OF
# THIS ONTOLOGY, EVEN IF ADVISED OF THE POSSIBILITY OF SUCH DAMAGE.
#

@prefix xsd:	<http://www.w3.org/2001/XMLSchema#> .
@prefix geo:	<http://www.w3.org/2003/01/geo/wgs84_pos#> .
@prefix dlpo:	<http://www.semanticdesktop.org/ontologies/2011/10/05/dlpo#> .
@prefix rdfs:    <http://www.w3.org/2000/01/rdf-schema#> .
@prefix nie:     <http://www.semanticdesktop.org/ontologies/2007/01/19/nie#> .
@prefix nrl:     <http://www.semanticdesktop.org/ontologies/2007/08/15/nrl#> .
@prefix nao:     <http://www.semanticdesktop.org/ontologies/2007/08/15/nao#> .
@prefix rdf:     <http://www.w3.org/1999/02/22-rdf-syntax-ns#> .
@prefix sioc: 	 <http://rdfs.org/sioc/ns#> .
@prefix sioct:   <http://rdfs.org/sioc/types#> .

<http://www.semanticdesktop.org/ontologies/2011/10/05/dlpo> {
	
	# Classes
	dlpo:LivePost
		a	rdfs:Class ;
		rdfs:comment "A generic representation of personal information intended for instant online sharing, typically over social networks. Extended through various subclasses. When an item is shared as a livepost, it can be managed as a separate new entity. For this purpose, all LivePost instances also become instances of nie:InformationElements." ;
		rdfs:subClassOf nie:InformationElement , sioc:Post ;
		rdfs:label "LivePost" .
						
	dlpo:MultimediaPost
		a	rdfs:Class ;
		rdfs:comment "A livepost consisting of a multimedia item, including links to online items. Further subclasses represent video, audio or image posts, as defined by various instances of the NFO (File Ontology)." ;
		rdfs:label "Multimedia Post" ;
		rdfs:subClassOf dlpo:LivePost .
	
	dlpo:VideoPost
		a	rdfs:Class ;
		rdfs:comment "Represents the live posting of a video file, or a link to an online media such as podcasts, videos, etc., as defined by instances of nfo:Video." ;
		rdfs:label "Video Post" ;
		rdfs:subClassOf dlpo:MultimediaPost .
	
	dlpo:AudioPost
		a	rdfs:Class ;
		rdfs:comment "Represents the live posting of audio file, or a link to online media such as podcasts, music, etc., as defined by instances of nfo:Audio." ;
		rdfs:label "Audio Post" ;
		rdfs:subClassOf dlpo:MultimediaPost .
		
	dlpo:ImagePost
		a	rdfs:Class ;
		rdfs:comment "Represents the live posting of an image file, or a link to an online image, as defined by instances of nfo:Image." ;
		rdfs:label "Image Post" ;
		rdfs:subClassOf dlpo:MultimediaPost .
		
	dlpo:PresencePost
		a	rdfs:Class ;
		rdfs:comment "A livepost consisting of information related to a user's presence, as defined by a set of DPO (Presence Ontology) instances." ;
		rdfs:label "Presence Post" ;
		rdfs:subClassOf dlpo:LivePost .
		
	dlpo:AvailabilityPost
		a	rdfs:Class ;
		rdfs:comment "Represents the live posting of information related to a user's detected or proclaimed availability, as defined by a set of instances of dpo:Availability." ;
		rdfs:label "Availability Post" ;
		rdfs:subClassOf dlpo:PresencePost .
		
	dlpo:ActivityPost
		a	rdfs:Class ;
		rdfs:comment "Represents the live posting of information related to a user's detected or proclaimed activity, as defined by a set of instances of dpo:Activity." ;
		rdfs:label "Activity Post" ;
		rdfs:subClassOf dlpo:PresencePost .	
			
	dlpo:EventPost
		a	rdfs:Class ;
		rdfs:comment "Represents the live posting of information related to a user's detected or proclaimed attendance in an ongoing event, as defined by an established instance of pimo:Event." ;
		rdfs:label "Event Post" ;
		rdfs:subClassOf dlpo:PresencePost .
		
	dlpo:Checkin
		a	rdfs:Class ;
		rdfs:comment "Represents the live posting of information related to a user's detected or proclaimed physical location, as defined by an established instance of pimo:Location." ;
		rdfs:label "Checkin Post" ;
		rdfs:subClassOf dlpo:PresencePost .	
		
	dlpo:Message
		a	rdfs:Class ;
		rdfs:comment "A livepost consisting of a textual message posted by either a user, or a contact, as defined by further subclasses." ;
		rdfs:label "Message" ;
		rdfs:subClassOf dlpo:LivePost .	
		
	dlpo:Status
		a	rdfs:Class ;
		rdfs:comment "Represents a status message, tweet, etc. shared by a user." ;
		rdfs:label "Status Message" ;
		rdfs:subClassOf dlpo:Message .	
	
	dlpo:Comment
		a	rdfs:Class ;
		rdfs:comment "Represents comments shared by a user or a contact, in reply to existing liveposts." ;
		rdfs:label "Comment" ;
		rdfs:subClassOf dlpo:Message, sioct:Comment .	
		
	dlpo:WebDocumentPost
		a	rdfs:Class ;
		rdfs:comment "A livepost consisting of links to remote web documents, as defined by further subclasses." ;
		rdfs:label "Web Document Post" ;
		rdfs:subClassOf dlpo:LivePost .
	
	dlpo:NotePost
		a	rdfs:Class ;
		rdfs:comment "Represents a livepost referring to an online note, as defined by instances of nfo:RemoteDataObject, or known instances of pimo:Note." ;
		rdfs:label "Note Post" ;
		rdfs:subClassOf dlpo:WebDocumentPost .
	
	dlpo:BlogPost
		a	rdfs:Class ;
		rdfs:comment "Represents a livepost referring to an online note, as defined by instances of nfo:RemoteDataObject, or known instances of pimo:Blogpost." ;
		rdfs:label "Blogpost" ;
		rdfs:subClassOf dlpo:WebDocumentPost, sioct:BlogPost .

	# Properties
	dlpo:hasReply
		a	rdf:Property ;
		rdfs:comment "Links a livepost to its reply or response, also in the form of a livepost. This property is transitive, and is the inverse of dlpo:replyOf." ;
		rdfs:domain dlpo:LivePost ;
		rdfs:label "has reply" ;
		rdfs:range dlpo:LivePost ;
		rdfs:subPropertyOf sioc:has_reply ;
		nrl:inverseProperty dlpo:replyOf .
		
	dlpo:replyOf
		a	rdf:Property ;
		rdfs:comment "Links an in-reply-to livepost to the original livepost. This property is transitive, and is the inverse of dlpo:hasReply." ;
		rdfs:domain dlpo:LivePost ;
		rdfs:label "reply of" ;
		rdfs:range dlpo:LivePost ;
		rdfs:subPropertyOf sioc:reply_of ;
		nrl:maxCardinality "1"^^xsd:nonNegativeInteger ;
		nrl:inverseProperty dlpo:hasReply .
		
	dlpo:hasRepost
		a	rdf:Property, nrl:TransitiveProperty ;
		rdfs:comment "Links to the repost(s) of a livepost. This property is transitive, and is the inverse of dlpo:repostOf." ;
		rdfs:domain dlpo:LivePost ;
		rdfs:label "has repost" ;
		rdfs:range dlpo:LivePost ;
		nrl:inverseProperty dlpo:repostOf .
		
	dlpo:repostOf
		a	rdf:Property, nrl:TransitiveProperty ;
		rdfs:comment "Links to the original of a reposted livepost. This property is transitive, and is the inverse of dlpo:hasRepost." ;
		rdfs:domain dlpo:LivePost ;
		rdfs:label "repost of" ;
		rdfs:range dlpo:LivePost ;
		nrl:maxCardinality "1"^^xsd:nonNegativeInteger ;
		nrl:inverseProperty dlpo:hasRepost .
		
	dlpo:isComposedOf
		a	rdf:Property ;
		rdfs:comment "One online post can simultaneously consist of various types of livepost subclasses as defined by DLPO. These are semantically related to the parent post through this property." ;
		rdfs:domain dlpo:LivePost ;
		rdfs:label "is composed of" ;
		rdfs:subPropertyOf nao:hasSubResource ;
		rdfs:range dlpo:LivePost .	
		
	dlpo:definingResource
		a	rdf:Property ;
		rdfs:comment "As many resources that are shared as liveposts exist beforehand, this property (a sub-property of nao:hasSuperResource) is provided to make this link explicit. Therefore a livepost (videopost, eventpost, availabilitypost, etc.) can be linked to the representation of the original resource being shared online (video, event, availability, etc.)"; 
		rdfs:domain	dlpo:LivePost ;
		rdfs:label	"has defining resource" ;
		rdfs:range	rdfs:Resource ;
		rdfs:subPropertyOf nao:hasSuperResource .
	
	dlpo:relatedResource
		a	rdf:Property ;
		rdfs:comment	"This property (a sub-property of nao:isRelated) is used to refer to resources that are related to the livepost, as opposed to being the resource being shared (refer to dlpo:definingResource). Typical uses for this property is to represent items (e.g. people) tagged to a livepost." ;
		rdfs:domain	dlpo:LivePost ;
		rdfs:label	"has related resource" ;
		rdfs:range	rdfs:Resource ;
		rdfs:subPropertyOf nao:isRelated .
		
	dlpo:timestamp
		a	rdf:Property ;
		rdfs:comment	"Records the time and date at which a Livepost is published at." ;
		rdfs:domain	dlpo:LivePost ;
		rdfs:label	"Timestamp" ;
		nrl:cardinality "1"^^xsd:nonNegativeInteger ;
		rdfs:range	xsd:datetime .
		
	dlpo:textualContent
		a	rdf:Property ;
		rdfs:comment	"The textual content of a Livepost, as it appears an online stream." ;
		rdfs:domain	dlpo:LivePost ;
		rdfs:label	"Textual Content" ;
		nrl:maxCardinality "1"^^xsd:nonNegativeInteger ;
		rdfs:range xsd:string .
}


<http://www.semanticdesktop.org/ontologies/2011/10/05/dlpo/metadata> {
    <http://www.semanticdesktop.org/ontologies/2011/10/05/dlpo/metadata>
          a       nrl:GraphMetadata ;
          nrl:coreGraphMetadataFor <http://www.semanticdesktop.org/ontologies/2011/10/05/dlpo> .

    <http://www.semanticdesktop.org/ontologies/2011/10/05/dlpo>
          a       nrl:Ontology , nrl:DocumentGraph ;
          nao:hasDefaultNamespace "http://www.semanticdesktop.org/ontologies/2011/10/05/dlpo#" ;
          nao:hasDefaultNamespaceAbbreviation "dlpo" ;
          nao:lastModified "2012-06-18T00:00:00Z" ;
          nao:serializationLanguage "TriG" ;
          nao:status "Recommendation" ;
          nrl:updatable "0" ;
		  nao:creator <http://www.deri.ie/about/team/member/simon_scerri> ;
		  nao:contributor <http://www.deri.ie/about/team/member/keith_cortis> ;
          nao:version "1.0" ;
          nao:prefLabel "digital.me LivePost Ontology" ;
          nao:description "The DLPO represents social interactions taking place within social networks, and all sorts of items that can conventionally be shared through them." .
}
