#
# Copyright (c) 2010 Evgeny Egorochkin <phreedom.stdin@gmail.com>
#
# All rights reserved, licensed under either CC-BY or BSD.
#
# You are free:
#  * to Share - to copy, distribute and transmit the work
#  * to Remix - to adapt the work
# Under the following conditions:
#  * Attribution - You must attribute the work in the manner specified by the author
#    or licensor (but not in any way that suggests that they endorse you or your use 
#    of the work).
#
# Redistribution and use in source and binary forms, with or without modification, 
# are permitted provided that the following conditions are met:
#  * Redistributions of source code must retain the above copyright notice, this 
#    list of conditions and the following disclaimer.
#  * Redistributions in binary form must reproduce the above copyright notice, this 
#    list of conditions and the following disclaimer in the documentation and/or 
#    other materials provided with the distribution.
#  * Neither the names of the authors nor the names of contributors may
#    be used to endorse or promote products derived from this ontology without 
#    specific prior written permission.
#
# THIS ONTOLOGY IS PROVIDED BY THE AUTHOR ``AS IS'' AND ANY EXPRESS OR
# IMPLIED WARRANTIES, INCLUDING, BUT NOT LIMITED TO, THE IMPLIED WARRANTIES
# OF MERCHANTABILITY AND FITNESS FOR A PARTICULAR PURPOSE ARE DISCLAIMED.
# IN NO EVENT SHALL THE AUTHOR BE LIABLE FOR ANY DIRECT, INDIRECT,
# INCIDENTAL, SPECIAL, EXEMPLARY, OR CONSEQUENTIAL DAMAGES (INCLUDING, BUT
# NOT LIMITED TO, PROCUREMENT OF SUBSTITUTE GOODS OR SERVICES; LOSS OF USE,
# DATA, OR PROFITS; OR BUSINESS INTERRUPTION) HOWEVER CAUSED AND ON ANY
# THEORY OF LIABILITY, WHETHER IN CONTRACT, STRICT LIABILITY, OR TORT
# (INCLUDING NEGLIGENCE OR OTHERWISE) ARISING IN ANY WAY OUT OF THE USE OF
# THIS ONTOLOGY, EVEN IF ADVISED OF THE POSSIBILITY OF SUCH DAMAGE.
#

@prefix rdf:     <http://www.w3.org/1999/02/22-rdf-syntax-ns#> .
@prefix rdfs:    <http://www.w3.org/2000/01/rdf-schema#> .
@prefix ndo:     <http://www.semanticdesktop.org/ontologies/2010/04/30/ndo#> .
@prefix nrl:     <http://www.semanticdesktop.org/ontologies/2007/08/15/nrl#> .
@prefix nuao:    <http://www.semanticdesktop.org/ontologies/2010/01/25/nuao#> .
@prefix nao:     <http://www.semanticdesktop.org/ontologies/2007/08/15/nao#> .
@prefix nmo:     <http://www.semanticdesktop.org/ontologies/2007/03/22/nmo#> .
@prefix nco:     <http://www.semanticdesktop.org/ontologies/2007/03/22/nco#> .
@prefix xsd:     <http://www.w3.org/2001/XMLSchema#> .
@prefix nie:     <http://www.semanticdesktop.org/ontologies/2007/01/19/nie#> .
@prefix nfo:     <http://www.semanticdesktop.org/ontologies/2007/03/22/nfo#> .

<http://www.semanticdesktop.org/ontologies/2010/04/30/ndo> {

    ndo:P2PFile
        a rdfs:Class ;
        rdfs:subClassOf nfo:RemoteDataObject;
        rdfs:label "P2P file" ;
        rdfs:comment "A file available via a peer-to-peer network" .

    ndo:TorrentedFile
        a rdfs:Class ;
        rdfs:subClassOf ndo:P2PFile;
        rdfs:label "torrented file" ;
        rdfs:comment "A file available via a BitTorrent peer-to-peer network" .

    ndo:Torrent
        a rdfs:Class;
        rdfs:subClassOf nie:InformationElement;
        rdfs:label "torrent" ;
        rdfs:comment "A .torrent file which contains references(ndo:TorrentedFile) to files available via BitTorrent. The references are pointed to via nie:hasLogicalPart" .

    ndo:DownloadEvent
        a rdfs:Class ;
        rdfs:subClassOf nuao:DesktopEvent ;
        rdfs:label "download event" ;
        rdfs:comment "A single event (from the point of view of the user) of downloading of a file or a set of files. Use nuao:involves to indicate the files involved. The event is assigned to downloaded copies of files. Can be assigned to multiple files." .

    ndo:copiedFrom
        a rdf:Property ;
        rdfs:label "copied from" ;
        rdfs:comment "Links a DataObject with its copy. This relation means that originally the Data Objects were copies but might have changed subsequentially." ;
        rdfs:domain nie:DataObject ;
        rdfs:range nie:DataObject .

    ndo:referrer
        a rdf:Property ;
        rdfs:label "referrer" ;
        rdfs:comment "Points to the Information Element that contained the link to the download source which was used in the download event." ;
        rdfs:domain ndo:DownloadEvent ;
        rdfs:range nie:InformationElement .
}

<http://www.semanticdesktop.org/ontologies/2010/04/30/ndo/metadata>
{
    <http://www.semanticdesktop.org/ontologies/2010/04/30/ndo>
          a       nrl:DocumentGraph , nrl:KnowledgeBase ;
          nao:hasDefaultNamespace "http://www.semanticdesktop.org/ontologies/2010/04/30/ndo#" ;
          nao:hasDefaultNamespaceAbbreviation "ndo" ;
          nao:lastModified "2010-04-30T09:38:49Z" ;
          nao:serializationLanguage "TriG" ;
          nao:status "Recommendation" ;
          nrl:updatable "0" ;
          nao:version "v1.0" ;
          nao:prefLabel "Nepomuk Download Ontology ";
          nao:description "The Nepomuk Download Ontology provides classes and properties to describe file downloads." .

    <http://www.semanticdesktop.org/ontologies/2010/04/30/ndo/metadata>
          a       nrl:GraphMetadata ;
          nao:serializationLanguage "TriG" ;
          nrl:coreGraphMetadataFor <http://www.semanticdesktop.org/ontologies/2010/04/30/ndo> .
}
