@prefix : <http://banshee-sympatico/percy#> .
@prefix owl: <http://www.w3.org/2002/07/owl#> .
@prefix rdf: <http://www.w3.org/1999/02/22-rdf-syntax-ns#> .
@prefix xml: <http://www.w3.org/XML/1998/namespace> .
@prefix xsd: <http://www.w3.org/2001/XMLSchema#> .
@prefix rdfs: <http://www.w3.org/2000/01/rdf-schema#> .
@base <http://banshee-sympatico/percy> .

<http://banshee-sympatico/percy> rdf:type owl:Ontology ;
                                  rdfs:comment "Percy is a UI to a set of underlying data which should be accessible at your fingertips. The interface is designed to quickly find exposed entities and provide a flexible set of actions which allows integrating to other systems. The common use is to search over web pages/resources and open them in the browser. This is similar to function to an autocomplete for a list of bookmarks." .

#################################################################
#    Data properties
#################################################################

###  http://banshee-sympatico/percy#title
:title rdf:type owl:DatatypeProperty ;
       rdfs:domain :Entity ;
       rdfs:range xsd:string ;
       rdfs:comment "Title of the entity. Should include any primary identifying information. For Jira issues, the issue key should be part of the title string." .


###  http://banshee-sympatico/percy#url
:url rdf:type owl:DatatypeProperty ;
     rdfs:domain :WebEntity ;
     rdfs:range xsd:string ;
     rdfs:comment "URL of a web resource. The web URL used to access the entity." .


#################################################################
#    Classes
#################################################################

###  http://banshee-sympatico/percy#Entity
:Entity rdf:type owl:Class .


###  http://banshee-sympatico/percy#Source
:Source rdf:type owl:Class .


###  http://banshee-sympatico/percy#WebEntity
:WebEntity rdf:type owl:Class ;
           rdfs:subClassOf :Entity .


###  Generated by the OWL API (version 4.5.9.2019-02-01T07:24:44Z) https://github.com/owlcs/owlapi
